wip

steel/Zeta.Steel.AggregateEpochHashes.fsti
@@ -1,41 +1,54 @@
 module Zeta.Steel.AggregateEpochHashes
 
 open FStar.Ghost
+open Steel.ST.Util
+module A = Steel.ST.Array
+module R = Steel.ST.Reference
+module G = Steel.ST.GhostReference
+module Lock = Steel.ST.SpinLock
 open Zeta.Steel.ApplicationTypes
 module U8 = FStar.UInt8
 module U16 = FStar.UInt16
 module U32 = FStar.UInt32
 module U64 = FStar.UInt64
 open Zeta.Steel.FormatsManual
-open Steel.Memory
-open Steel.Effect.Atomic
-open Steel.Effect
-open Steel.Reference
-open Steel.Array
-module IArray = Steel.Hashtbl
+module IArray = Zeta.Steel.IArray
 module T = Zeta.Steel.FormatsManual
 module M = Zeta.Steel.ThreadStateModel
-module A = Steel.Array
-module Lock = Steel.SpinLock
 module HA = Zeta.Steel.HashAccumulator
+open Zeta.Steel.Util
 #push-options "--ide_id_info_off"
 
+/// Initializer for an IArray
 val epoch_hash_size : U32.t
 
-let log_ref = ghost_ref (Seq.seq log_entry_base)
-
+let log_ref = G.ref (Seq.seq log_entry_base)
 let log_refs_t = Map.t thread_id log_ref
 
-let hash_value = u256 & U64.t
 let zero_hash : HA.hash_value_t = HA.initial_hash
 let related_hashes (h:hash_value) (h':HA.hash_value_t) = True // TODO
 
 noeq
-type epoch_hash_t = {
-  hadd: hash_value;
-  hevict: hash_value;
-  certified: bool;
+type epoch_hashes_t = {
+  hadd: HA.ha;
+  hevict: HA.ha;
+  complete: erased bool;
 }
+
+let epoch_hashes_repr = IArray.repr M.epoch_id M.epoch_hash
+let epoch_id_hash (x:M.epoch_id) : U32.t = x
+let epoch_hash_perm (k:M.epoch_id) (v:epoch_hashes_t) (c:M.epoch_hash) =
+    HA.ha_val v.hadd c.hadd `star`
+    HA.ha_val v.hevict c.hevict `star`
+    pure (reveal v.complete == c.epoch_complete)
+
+let all_epoch_hashes =
+  IArray.tbl
+    #M.epoch_id
+    #epoch_hashes_t
+    #M.epoch_hash
+    epoch_id_hash
+    epoch_hash_perm
 
 let related (h h':M.epoch_hash) =
    (if h'.epoch_complete
@@ -45,16 +58,14 @@ let related (h h':M.epoch_hash) =
       h.hevict == zero_hash
    ))
 
-let epoch_id_hash = fun (e:M.epoch_id) -> e
-let epoch_hashes_t = IArray.tbl M.epoch_id epoch_hash_t epoch_id_hash
 let epoch_hash_contributions_t = Map.t (thread_id & M.epoch_id) M.epoch_hash
 
-let all_contributions_are_accurate (_:IArray.repr M.epoch_id epoch_hash_t)
+let all_contributions_are_accurate (_:epoch_hashes_repr)
                                    (_:epoch_hash_contributions_t)
   : prop
   = True //TODO
 
-let max_certified_epoch_is (_:IArray.repr M.epoch_id epoch_hash_t)
+let max_certified_epoch_is (_:epoch_hashes_repr)
                            (_:M.epoch_id)
   : prop
   = True //TODO
@@ -67,36 +78,45 @@ let per_thread_contribiution_is_accurate (tid:thread_id)
     forall (eid:M.epoch_id). related (Map.sel contribs (tid, eid))
                                 (Map.sel tsm.epoch_hashes eid)
 
-let full = Steel.FractionalPermission.full_perm
-let half = Steel.FractionalPermission.half_perm full
-val h_forall (#a:Type u#a) (f: a -> vprop) : vprop
+
+let rec forall_threads_between (tid:thread_id)
+                               (down_to:thread_id { U16.v tid >= U16.v down_to })
+                               (f:thread_id -> vprop)
+  : Tot (vprop)
+        (decreases (U16.v tid))
+  = f tid `star`
+    (if tid = down_to then emp
+     else forall_threads_between U16.(tid -^ 1us) down_to f)
+
+let forall_threads (f:thread_id -> vprop) =
+  forall_threads_between
+    (UInt16.uint_to_t (U32.v n_threads))
+    0us
+    f
+
 
 let lock_inv (log_refs:log_refs_t)
-             (hashes : epoch_hashes_t)
-             (max_certified_epoch : ref M.epoch_id)
-             (contributions: ghost_ref epoch_hash_contributions_t)
+             (hashes : all_epoch_hashes)
+             (max_certified_epoch : R.ref M.epoch_id)
+             (contributions: G.ref epoch_hash_contributions_t)
  : vprop
- = h_exists (fun (hashes_v, max, contributions_v) ->
-      IArray.tpts_to hashes hashes_v `star`
-      pts_to max_certified_epoch full max `star`
-      ghost_pts_to contributions full contributions_v `star`
+ = exists_ (fun (hashes_v, max, contributions_v) ->
+      IArray.perm hashes hashes_v Set.empty `star`
+      R.pts_to max_certified_epoch full max `star`
+      G.pts_to contributions full contributions_v `star`
       pure (all_contributions_are_accurate hashes_v contributions_v /\
             max_certified_epoch_is hashes_v max) `star`
-      h_forall (fun (tid:thread_id) ->
-        if Map.contains log_refs tid
-        then (
-          let logref = Map.sel log_refs tid in
-          h_exists (fun (entries:_) ->
-            ghost_pts_to logref half entries `star`
+      forall_threads (fun (tid:thread_id) ->
+        let logref = Map.sel log_refs tid in
+        exists_ (fun (entries:_) ->
+            G.pts_to logref half entries `star`
             pure (per_thread_contribiution_is_accurate tid entries contributions_v))
-        )
-        else emp
       ))
 
 noeq
 type aggregate_epoch_hashes (log_refs:log_refs_t) = {
-     hashes : epoch_hashes_t;
-     max_certified_epoch : ref M.epoch_id;
-     contributions: ghost_ref epoch_hash_contributions_t;
+     hashes : all_epoch_hashes;
+     max_certified_epoch : R.ref M.epoch_id;
+     contributions: G.ref epoch_hash_contributions_t;
      lock: Lock.lock (lock_inv log_refs hashes max_certified_epoch contributions)
 }
