steel/Zeta.Steel.Verifier.fsti
@@ -1,96 +1,93 @@
 module Zeta.Steel.Verifier
 include Zeta.Steel.VerifierTypes
 open FStar.Ghost
+open Steel.ST.Util
+module G = Steel.ST.GhostReference
+module R = Steel.ST.Reference
+module A = Steel.ST.Array
 open Zeta.Steel.ApplicationTypes
 module U8 = FStar.UInt8
 module U16 = FStar.UInt16
 module U32 = FStar.UInt32
 module U64 = FStar.UInt64
 open Zeta.Steel.FormatsManual
-open Steel.Memory
-open Steel.Effect.Atomic
-open Steel.Effect
-open Steel.Reference
-open Steel.Array
-
+open Zeta.Steel.Util
 module T = Zeta.Steel.FormatsManual
 module M = Zeta.Steel.ThreadStateModel
-module A = Steel.Array
 module AEH = Zeta.Steel.AggregateEpochHashes
+module P = Zeta.Steel.Parser
 
 #push-options "--ide_id_info_off"
 
-val spec_parser_log : Zeta.Steel.Parser.spec_parser (Seq.seq log_entry_base)
+val spec_parser_log : P.spec_parser (Seq.seq log_entry_base)
+
+let parse_log (l:bytes) =
+  match spec_parser_log l with
+  | None -> None
+  | Some (v, n) ->
+    if n = Seq.length l
+    then Some v
+    else None
 
 val create (tid:T.thread_id)
-  : Steel thread_state_t
+  : STT thread_state_t
     emp
-    (fun t -> thread_state_inv t)
-    (requires fun h -> True)
-    (ensures fun _ vs h1 ->
-      value_of vs h1 == M.init_thread_state_model tid)
+    (fun t -> thread_state_inv t (M.init_thread_state_model tid))
 
-module P = Zeta.Steel.Parser
+let delta_app_results (tsm0 tsm1:M.thread_state_model)
+  : GTot (Seq.seq M.app_results)
+  = Prims.admit()
 
-val serialized_new_app_results (init final:M.app_results)
-                               (n_out:U32.t)
-                               (out: P.bytes)
-  : prop
+let bytes_of_app_results (s:Seq.seq M.app_results)
+  : GTot bytes
+  = Prims.admit()
 
-let log_entries = Seq.seq log_entry_base
-
-let committed_prefix (l0 l1:log_entries) : prop = True
-
-[@@ __steel_reduce__]
-let ghost_sel (#a:Type)
-              (#p:vprop)
-              (q:Steel.FractionalPermission.perm)
-              (r:ghost_ref a)
-              (h:rmem p{
-                FStar.Tactics.with_tactic
-                  selector_tactic
-                  (can_be_split p (ghost_vptrp r q) /\ True)
-              })
-  = h (ghost_vptrp r q)
-
-val verify (t:thread_state_t)
-           (len:U32.t) (log:A.array U8.t)
-           (outlen:U32.t) (out:A.array U8.t)
-           (logrefs: erased (AEH.log_refs_t))
-           (aeh:AEH.aggregate_epoch_hashes logrefs)
-           (mylogref:AEH.log_ref)
-  : Steel U32.t
-    (thread_state_inv t `star`
-     (A.varray log `star`
-      A.varray out `star`
-      ghost_vptrp mylogref AEH.half))
-    (fun _ ->
-      thread_state_inv t `star`
-      (A.varray log `star`
-       A.varray out `star`
-       ghost_vptrp mylogref AEH.half))
-    (requires fun h ->
-      let tsm = value_of t (focus_rmem h _) in
-      let committed_entries = ghost_sel AEH.half mylogref h in
-      U32.v len == A.length log /\
-      U32.v outlen = A.length out /\
-      Map.sel logrefs tsm.thread_id == mylogref  /\
-      committed_prefix committed_entries tsm.processed_entries
-      )
-    (ensures fun h0 n_out h1 ->
-      let tsm0 = value_of t (focus_rmem h0 _) in
-      let tsm1 = value_of t (focus_rmem h1 _) in
-      let log_bytes = A.asel log h0 in
-      let out_bytes = A.asel out h1 in
-      let committed_entries = ghost_sel AEH.half mylogref h1 in
-      log_bytes == A.asel log h1 /\ //log unchanged
-      (match spec_parser_log log_bytes with
-       | None -> tsm1.failed
-       | Some (log_entries, n) ->
-         if n = U32.v len
-         then ( //parsing succeeded
-           tsm1 == M.verify_model tsm0 log_entries /\
-           serialized_new_app_results tsm0.app_results tsm1.app_results n_out out_bytes /\
-           committed_prefix tsm1.processed_entries committed_entries
-         )
-         else tsm1.failed))
+/// Entry point to run a single verifier thread on a log
+val verify (#tsm:M.thread_state_model)
+           (t:thread_state_t) //handle to the thread state
+           (#log_bytes:erased bytes)
+           (#len:U32.t)
+           (log:larray U8.t len) //concrete log
+           (#outlen:U32.t)
+           (out:larray U8.t outlen) //out array, to write outputs
+           (#logrefs: erased (AEH.log_refs_t))
+           (aeh:AEH.aggregate_epoch_hashes logrefs) //lock & handle to the aggregate state
+           (mylogref:AEH.log_ref { //this thread's contribution to the aggregate state
+             Map.sel logrefs tsm.thread_id == mylogref
+            })
+  : STT (option U32.t)
+    (//precondition
+      thread_state_inv t tsm `star` //thread state is initially tsm
+      A.pts_to log log_bytes `star` //the log contains log_bytes
+      exists_ (A.pts_to out) `star` //we have permission to out, don't care what it contains
+      G.pts_to mylogref half (M.committed_entries tsm) //and mylogref contains this thread's committed entries
+    )
+    (fun res -> //postcondition
+      A.pts_to log log_bytes `star` //log contents didn't change
+      (match res with
+       | None ->
+         //if it fails, you still get back ownership on the various
+         //resources, e.g., to free them
+         //but not much else
+         exists_ (thread_state_inv t) `star`
+         exists_ (A.pts_to out) `star`
+         exists_ (G.pts_to mylogref half)
+      | Some n_out ->
+         //it succeeded
+         exists_ (fun (tsm':M.thread_state_model) ->
+         exists_ (fun (out_bytes:Seq.seq U8.t) ->
+           thread_state_inv t tsm' `star` //tsm' is the new state of the thread
+           A.pts_to out out_bytes `star`  //the out array contains out_bytes
+           G.pts_to mylogref half (M.committed_entries tsm') `star` //my contributions are updated
+           pure (
+             match parse_log log_bytes with
+             | None -> False //log parsing did not fail
+             | Some log_entries -> //parsing produces log_entries
+               //tsm' what you get by running the spec verifier from tsm on log_entries
+               tsm' == M.verify_model tsm log_entries /\
+               //the out_bytes contain any new app results in tsm'
+               out_bytes == bytes_of_app_results (delta_app_results tsm tsm') /\
+               //and n_out is the number of bytes that were written
+               U32.v n_out == Seq.length out_bytes
+           )
+           ))))
