utils/Zeta.SeqAux.fsti
@@ -58,11 +58,11 @@ val lemma_prefix_create (#a:Type) (n:nat) (v:a) (i:nat{i <= n})
 : Lemma (prefix (create n v) i == create i v)
 
 (* is ps a prefix of s *)
-let is_prefix (#a:eqtype) (s:seq a) (ps: seq a): Tot bool =
-length ps <= length s &&
-ps = prefix s (length ps)
+let is_prefix (#a:Type) (s:seq a) (ps: seq a): Type0 =
+  length ps <= length s /\
+  ps == prefix s (length ps)
 
-let prefix_of (#a:eqtype) (s0 s1:seq a) = is_prefix s1 s0
+let prefix_of (#a:Type) (s0 s1:seq a) = is_prefix s1 s0
 
 (* Suffix of a sequence *)
 val suffix (#a:Type) (s:seq a) (i:nat{i <= length s}): Tot (s':seq a{length s' = i})
@@ -73,16 +73,16 @@ Lemma (requires (True))
       [SMTPat (index (suffix s i) j)]
 
 (* projection - a subsequence of the original sequence *)
-val proj (#a:eqtype): seq a -> seq a -> Type0
+val proj (#a:Type u#a): seq a -> seq a -> Type u#a
 
 (* mapping from a subsequence index to the corresponding index in the base sequence *)
-val proj_index_map (#a:eqtype) (ss: seq a) (s: seq a) (prf: proj ss s) (i:seq_index ss):
-Tot (j:seq_index s{index s j = index ss i})
+val proj_index_map (#a:Type) (ss: seq a) (s: seq a) (prf: proj ss s) (i:seq_index ss):
+Tot (j:seq_index s{index s j == index ss i})
 
-let proj_index_map_exists (#a:eqtype) (ss: seq a) (s: seq a{proj ss s}) (i:seq_index ss)
-: Lemma (exists (j:seq_index s). index s j = index ss i)
+let proj_index_map_exists (#a:Type) (ss: seq a) (s: seq a{proj ss s}) (i:seq_index ss)
+: Lemma (exists (j:seq_index s). index s j == index ss i)
 = let p : squash (proj ss s) = FStar.Squash.get_proof (proj ss s) in
-  let _ : squash (exists (j:seq_index s). index s j = index ss i) = 
+  let _ : squash (exists (j:seq_index s). index s j == index ss i) = 
     FStar.Squash.bind_squash p (fun p -> 
       let k = proj_index_map ss s p i in
       assert (index s k == index ss i))
@@ -90,57 +90,57 @@ let proj_index_map_exists (#a:eqtype) (ss: seq a) (s: seq a{proj ss s}) (i:seq_i
   ()
 
 (* the mapping we construct above is monotonic *)
-val lemma_proj_monotonic (#a:eqtype) (ss s: seq a) (prf: proj ss s) (i1 i2: seq_index ss):
+val lemma_proj_monotonic (#a:Type) (ss s: seq a) (prf: proj ss s) (i1 i2: seq_index ss):
 Lemma (requires (i1 < i2))
       (ensures (proj_index_map ss s prf i1 < proj_index_map ss s prf i2))
 
-val lemma_proj_length (#a:eqtype) (ss: seq a) (s:seq a{proj ss s}):
+val lemma_proj_length (#a:Type) (ss: seq a) (s:seq a{proj ss s}):
 Lemma (requires (True))
       (ensures (length ss <= length s))
 
 (* subsequence of s obtained by applying a filter *)
-val filter (#a:eqtype) (f:a -> bool) (s:seq a): Tot (seq a)
+val filter (#a:Type) (f:a -> bool) (s:seq a): Tot (seq a)
 
 (* filter is a projection *)
-val lemma_filter_is_proj (#a:eqtype) (f:a -> bool) (s:seq a):
-Lemma (proj (filter f s) s)
+val lemma_filter_is_proj (#a:Type) (f:a -> bool) (s:seq a)
+  : squash (proj (filter f s) s)
 
 (* constructive version of the lemma_filter_is_proj *)
-val filter_is_proj_prf (#a:eqtype) (f:a -> bool) (s:seq a): Tot (proj (filter f s) s)
+val filter_is_proj_prf (#a:Type) (f:a -> bool) (s:seq a): Tot (proj (filter f s) s)
 
 (* every index in the filtered sequence satisfies the filter predicate *)
-val lemma_filter_correct1 (#a: eqtype) (f:a -> bool) (s:seq a) (i:seq_index (filter f s)):
+val lemma_filter_correct1 (#a: Type) (f:a -> bool) (s:seq a) (i:seq_index (filter f s)):
 Lemma (requires (True))
       (ensures (f (index (filter f s) i) = true))
       [SMTPat (f (index (filter f s) i))]
 
-val lemma_filter_correct_all (#a:eqtype) (f:a -> bool) (s:seq a):
+val lemma_filter_correct_all (#a:Type) (f:a -> bool) (s:seq a):
 Lemma (requires (True))
       (ensures (forall (i:(seq_index (filter f s))). f (index (filter f s) i) = true))
 
-val lemma_filter_all_not (#a:eqtype) (f:a -> bool) (s:seq a):
+val lemma_filter_all_not (#a:Type) (f:a -> bool) (s:seq a):
 Lemma (requires filter f s `equal` empty)
       (ensures forall (i:seq_index s). not (f (index s i)))
 
-val lemma_filter_all_not_inv (#a:eqtype) (f:a->bool) (s:seq a)
+val lemma_filter_all_not_inv (#a:Type) (f:a->bool) (s:seq a)
 : Lemma (requires (forall (i:seq_index s). not (f (index s i))))
         (ensures (equal (filter f s) empty))
 
-val lemma_filter_exists (#a:eqtype) (f:a -> bool) (s:seq a):
+val lemma_filter_exists (#a:Type) (f:a -> bool) (s:seq a):
 Lemma (requires (exists (i:seq_index s). f (index s i)))
       (ensures (length (filter f s) > 0))
 
-val lemma_filter_unique (#a:eqtype) (f:a->bool) (s: seq a) (i:seq_index s)
+val lemma_filter_unique (#a:Type) (f:a->bool) (s: seq a) (i:seq_index s)
 : Lemma (requires (f (index s i) /\ (forall j. j <> i ==> not (f (index s j)))))
-        (ensures (filter f s = create 1 (index s i)))
+        (ensures (filter f s == create 1 (index s i)))
 
 (* mapping from filtered subseq to satisfying indexes *)
-val filter_index_map (#a:eqtype) (f:a -> bool) (s:seq a) (i:seq_index (filter f s)):
-Tot (j:seq_index s{index s j = index (filter f s) i})
+val filter_index_map (#a:Type) (f:a -> bool) (s:seq a) (i:seq_index (filter f s)):
+Tot (j:seq_index s{index s j == index (filter f s) i})
 
 (* Mapping from original seq to filtered subseq for satisfying indexes *)
-val filter_index_inv_map (#a:eqtype) (f:a -> bool) (s:seq a) (i:seq_index s{f (index s i)}):
-Tot (j:seq_index (filter f s){index s i = index (filter f s) j})
+val filter_index_inv_map (#a:Type) (f:a -> bool) (s:seq a) (i:seq_index s{f (index s i)}):
+Tot (j:seq_index (filter f s){index s i == index (filter f s) j})
 
 inline_for_extraction
 let refine #a (f:a -> bool) = x:a{f x}
@@ -162,174 +162,174 @@ Lemma (requires True)
       (ensures (index (seq_refine f s) i == index s i))
       [SMTPat (index (seq_refine f s) i)]
 
-let filter_refine (#a:eqtype) (f:a -> bool) (s: seq a): Tot (seq (refine f)) =
+let filter_refine (#a:Type) (f:a -> bool) (s: seq a): Tot (seq (refine f)) =
 let fs = filter f s in
 seq_refine f fs
 
 (* filter_index_map is injective *)
-val lemma_filter_index_map_monotonic (#a:eqtype) (f:a -> bool) (s:seq a)
+val lemma_filter_index_map_monotonic (#a:Type) (f:a -> bool) (s:seq a)
 (i:seq_index (filter f s))(j:seq_index (filter f s){j > i}):
 Lemma (filter_index_map f s i < filter_index_map f s j)
 
 (* Inverse mapping is injective *)
-val lemma_filter_index_inv_map_monotonic (#a:eqtype) (f:a -> bool) (s: seq a)
+val lemma_filter_index_inv_map_monotonic (#a:Type) (f:a -> bool) (s: seq a)
 (i:seq_index s) (j: seq_index s {j > i}):
     Lemma (requires (f (index s i) /\ f (index s j)))
           (ensures (filter_index_inv_map f s i < filter_index_inv_map f s j))
 
-val lemma_filter_maps_correct (#a:eqtype) (f:a -> bool) (s: seq a) (i:seq_index s):
+val lemma_filter_maps_correct (#a:Type) (f:a -> bool) (s: seq a) (i:seq_index s):
   Lemma (requires (f (index s i)))
         (ensures (filter_index_map f s (filter_index_inv_map f s i) = i))
 
-val lemma_filter_maps_correct2 (#a:eqtype) (f:a -> bool) (s: seq a) (i: seq_index (filter f s)):
+val lemma_filter_maps_correct2 (#a:Type) (f:a -> bool) (s: seq a) (i: seq_index (filter f s)):
   Lemma (requires(True))
         (ensures (filter_index_inv_map f s (filter_index_map f s i) = i))
         [SMTPat (filter_index_map f s i)]
 
-val lemma_filter_empty (#a:eqtype) (f:a -> bool):
+val lemma_filter_empty (#a:Type) (f:a -> bool):
   Lemma (filter f (empty #a) == empty #a)
 
-val lemma_filter_prefix (#a:eqtype) (f:a -> bool) (s: seq a) (ps: seq a{is_prefix s ps}):
+val lemma_filter_prefix (#a:Type) (f:a -> bool) (s: seq a) (ps: seq a{is_prefix s ps}):
   Lemma (is_prefix (filter f s) (filter f ps))
 
-val lemma_filter_prefix_comm (#a:eqtype) (f:a->bool) (s: seq a) (i:seq_index s):
+val lemma_filter_prefix_comm (#a:Type) (f:a->bool) (s: seq a) (i:seq_index s):
   Lemma (requires (f (index s i)))
-        (ensures (filter f (prefix s i) = prefix (filter f s) (filter_index_inv_map f s i)))
+        (ensures (filter f (prefix s i) == prefix (filter f s) (filter_index_inv_map f s i)))
 
-val lemma_filter_prefix_comm2 (#a:eqtype) (f:a->bool) (s: seq a) (i:seq_index s):
+val lemma_filter_prefix_comm2 (#a:Type) (f:a->bool) (s: seq a) (i:seq_index s):
   Lemma (requires (f (index s i)))
-        (ensures (filter f (prefix s (i+1)) = prefix (filter f s) (1 + (filter_index_inv_map f s i))))
+        (ensures (filter f (prefix s (i+1)) == prefix (filter f s) (1 + (filter_index_inv_map f s i))))
 
-val lemma_filter_extend1 (#a:eqtype) (f:a -> bool) (s:seq a{length s > 0}):
+val lemma_filter_extend1 (#a:Type) (f:a -> bool) (s:seq a{length s > 0}):
   Lemma (requires (not (f (index s (length s - 1)))))
-        (ensures (filter f s = filter f (prefix s (length s - 1))))
+        (ensures (filter f s == filter f (prefix s (length s - 1))))
 
-val lemma_filter_extend2 (#a:eqtype) (f:a -> bool) (s:seq a{length s > 0}):
+val lemma_filter_extend2 (#a:Type) (f:a -> bool) (s:seq a{length s > 0}):
   Lemma (requires (f (index s (length s - 1))))
-        (ensures (filter f s = append1 (filter f (prefix s (length s - 1))) (index s (length s - 1))))
+        (ensures (filter f s == append1 (filter f (prefix s (length s - 1))) (index s (length s - 1))))
 
-val lemma_filter_update_length (#a:eqtype) (f:a -> bool) (s:seq a) (i:seq_index s) (v:a)
-  : Lemma (requires (f v = f (index s i)))
+val lemma_filter_update_length (#a:Type) (f:a -> bool) (s:seq a) (i:seq_index s) (v:a)
+  : Lemma (requires (f v == f (index s i)))
           (ensures (length (filter f s) = length (filter f (upd s i v))))
           [SMTPat (length (filter f (upd s i v)))]
 
-val lemma_filter_update_index_eq (#a:eqtype) (f:a -> bool) (s:seq a) (i:seq_index s) (v:a)
+val lemma_filter_update_index_eq (#a:Type) (f:a -> bool) (s:seq a) (i:seq_index s) (v:a)
   : Lemma (requires (f v /\ f (index s i)))
-          (ensures (index (filter f (upd s i v)) (filter_index_inv_map f s i) = v))
+          (ensures (index (filter f (upd s i v)) (filter_index_inv_map f s i) == v))
 
 (*
-val lemma_filter_update_index_neq (#a:eqtype) (f:a -> bool) (s:seq a) (i:seq_index s) (v:a) (j:seq_index (filter f s))
+val lemma_filter_update_index_neq (#a:Type) (f:a -> bool) (s:seq a) (i:seq_index s) (v:a) (j:seq_index (filter f s))
   : Lemma (requires (f v = f (index s i) /\ filter_index_map f s j <> i))
           (ensures (index (filter f s) j = index (filter f (upd s i v)) j))
 *)
 
-let ext_pred (#a:eqtype) (f1 f2:a -> bool) =
+let ext_pred (#a:Type) (f1 f2:a -> bool) =
   forall x. f1 x = f2 x
 
-val lemma_filter_extensionality (#a:eqtype) (f1 f2:a -> bool) (s:seq a):
+val lemma_filter_extensionality (#a:Type) (f1 f2:a -> bool) (s:seq a):
   Lemma (requires (ext_pred f1 f2))
-        (ensures (filter f1 s = filter f2 s))
+        (ensures (filter f1 s == filter f2 s))
 
-let conj (#a:eqtype) (f1 f2: a -> bool) (x: a) =
+let conj (#a:Type) (f1 f2: a -> bool) (x: a) =
   f1 x && f2 x
 
-val lemma_filter_conj (#a:eqtype) (f1 f2: a -> bool) (s:seq a):
-  Lemma (filter (conj f1 f2) s = filter f1 (filter f2 s))
+val lemma_filter_conj (#a:Type) (f1 f2: a -> bool) (s:seq a):
+  Lemma (filter (conj f1 f2) s == filter f1 (filter f2 s))
 
-val lemma_filter_comm (#a:eqtype) (f1 f2:a -> bool) (s:seq a):
-  Lemma (filter f2 (filter f1 s) = filter f1 (filter f2 s))
+val lemma_filter_comm (#a:Type) (f1 f2:a -> bool) (s:seq a):
+  Lemma (filter f2 (filter f1 s) == filter f1 (filter f2 s))
 
 (* The index of the last entry that satisfies a given property *)
-val last_index_opt (#a:eqtype) (f:a -> bool) (s:seq a):
+val last_index_opt (#a:Type) (f:a -> bool) (s:seq a):
   Tot (option (i:seq_index s{f (index s i)}))
 
 (* There exists some element satisfying f if there exists last_index *)
-let exists_sat_elems (#a:eqtype) (f:a -> bool) (s:seq a) =
+let exists_sat_elems (#a:Type) (f:a -> bool) (s:seq a) =
   Some? (last_index_opt f s)
 
 (* The index of the last entry when we know there exists such entry *)
-let last_index (#a:eqtype) (f:a -> bool) (s:seq a{exists_sat_elems f s}) =
+let last_index (#a:Type) (f:a -> bool) (s:seq a{exists_sat_elems f s}) =
   Some?.v (last_index_opt f s)
   
 (* Any index beyond last index does not satisfy f *)
-val lemma_last_index_correct1 (#a:eqtype) (f:a -> bool) (s:seq a) (i:seq_index s):
+val lemma_last_index_correct1 (#a:Type) (f:a -> bool) (s:seq a) (i:seq_index s):
   Lemma (requires (exists_sat_elems f s /\ i > last_index f s))
         (ensures (not (f (index s i))))
 
 (* Any witness satisfying f implies last_index exists *)
-val lemma_last_index_correct2 (#a:eqtype) (f:a -> bool) (s:seq a) (i:seq_index s):
+val lemma_last_index_correct2 (#a:Type) (f:a -> bool) (s:seq a) (i:seq_index s):
   Lemma (requires (f (index s i)))
         (ensures (exists_sat_elems f s /\ last_index f s >= i))
 
-val last_index_opt_elim (#a:eqtype) (f:a → bool) (s:seq a)
+val last_index_opt_elim (#a:Type) (f:a → bool) (s:seq a)
   : Lemma (match last_index_opt f s with
            | None → ∀ (i:seq_index s). not (f (Seq.index s i))
            | Some i → f (Seq.index s i) ∧ (∀ (j:seq_index s). j > i ⟹ not (f (Seq.index s j))))
 
 (* Taking the prefix of a sequence upto last_index does not alter last_index *)
-val lemma_last_index_prefix (#a:eqtype) (f:a -> bool) (s:seq a) (i:nat{i <= length s}):
+val lemma_last_index_prefix (#a:Type) (f:a -> bool) (s:seq a) (i:nat{i <= length s}):
   Lemma (requires (exists_sat_elems f s /\ i > last_index f s))
         (ensures (exists_sat_elems f (prefix s i) /\
                   last_index f s = last_index f (prefix s i)))
 
 (* If s does not have elements satisfying f then no prefix of s has as well *)
-val lemma_not_exists_prefix (#a:eqtype) (f:a -> bool) (s:seq a) (i:nat{i <= length s}):
+val lemma_not_exists_prefix (#a:Type) (f:a -> bool) (s:seq a) (i:nat{i <= length s}):
   Lemma (requires (not (exists_sat_elems f s)))
         (ensures (not (exists_sat_elems f (prefix s i))))
 
-val lemma_exists_sat_elems_exists (#a:eqtype) (f:a -> bool) (s:seq a)
+val lemma_exists_sat_elems_exists (#a:Type) (f:a -> bool) (s:seq a)
   : Lemma (exists_sat_elems f s <==> (exists (i:seq_index s). f (Seq.index s i)))
   
-val lemma_exists_prefix_implies_exists (#a:eqtype) (f:a -> bool) (s:seq a) (i:nat{i <= length s}):
+val lemma_exists_prefix_implies_exists (#a:Type) (f:a -> bool) (s:seq a) (i:nat{i <= length s}):
   Lemma (requires (exists_sat_elems f (prefix s i)))
         (ensures (exists_sat_elems f s))
         [SMTPat (exists_sat_elems f (prefix s i))]
   
-val lemma_last_index_last_elem_nsat (#a:eqtype) (f:a -> bool) (s:seq a{length s > 0}):
+val lemma_last_index_last_elem_nsat (#a:Type) (f:a -> bool) (s:seq a{length s > 0}):
   Lemma (requires (not (f (index s (length s - 1)))))
         (ensures ((exists_sat_elems f s ==> last_index f s < length s - 1) /\
                   exists_sat_elems f s = exists_sat_elems f (prefix s (length s - 1))))
 
-val lemma_last_index_opt_last_elem_nsat (#a:eqtype) (f:a -> bool) (s:seq a{length s > 0}):
+val lemma_last_index_opt_last_elem_nsat (#a:Type) (f:a -> bool) (s:seq a{length s > 0}):
   Lemma (requires (not (f (index s (length s - 1)))))
         (ensures (match last_index_opt f s, last_index_opt f (prefix s (length s - 1)) with
                   | None, None -> True
                   | Some v0, Some v1 -> v0 == v1
                   | _ -> False))
 
-val lemma_last_index_last_elem_sat (#a:eqtype) (f:a -> bool) (s:seq a{length s > 0}):
+val lemma_last_index_last_elem_sat (#a:Type) (f:a -> bool) (s:seq a{length s > 0}):
   Lemma (requires (f (index s (length s - 1))))
         (ensures (exists_sat_elems f s /\ last_index f s = length s - 1))
 
-val lemma_exists_sat_elems_extensionality (#a:eqtype) (f1 f2:a -> bool) (s: seq a):
+val lemma_exists_sat_elems_extensionality (#a:Type) (f1 f2:a -> bool) (s: seq a):
   Lemma (requires (ext_pred f1 f2))
         (ensures (exists_sat_elems f1 s = exists_sat_elems f2 s))
 
-val lemma_last_index_extensionality (#a:eqtype) (f1 f2:a -> bool) (s: seq a{exists_sat_elems f1 s}):
+val lemma_last_index_extensionality (#a:Type) (f1 f2:a -> bool) (s: seq a{exists_sat_elems f1 s}):
   Lemma (requires (ext_pred f1 f2))
         (ensures (exists_sat_elems f2 s /\
                   last_index f1 s = last_index f2 s))
 
-val lemma_exists_sat_conj (#a:eqtype) (f1 f2: a -> bool) (s: seq a):
+val lemma_exists_sat_conj (#a:Type) (f1 f2: a -> bool) (s: seq a):
   Lemma(requires True)
        (ensures (exists_sat_elems (conj f1 f2) s = exists_sat_elems f1 (filter f2 s)))
        [SMTPat (exists_sat_elems (conj f1 f2) s)]
 
-val lemma_last_idx_conj (#a:eqtype) (f1 f2: a -> bool)
+val lemma_last_idx_conj (#a:Type) (f1 f2: a -> bool)
                         (s: seq a{exists_sat_elems (conj f1 f2) s}):
   Lemma (last_index (conj f1 f2) s = filter_index_map f2 s (last_index f1 (filter f2 s)))
 
 (* The index of the first entry that satisfies a given property *)
-val first_index (#a:eqtype) (f:a -> bool) (s:seq a{exists_sat_elems f s})
+val first_index (#a:Type) (f:a -> bool) (s:seq a{exists_sat_elems f s})
   : Tot (i:seq_index s{f (index s i)})
 
 (* Any index before first index does not satisfy f *)
-val lemma_first_index_correct1 (#a:eqtype) (f:a -> bool) (s:seq a) (i:seq_index s):
+val lemma_first_index_correct1 (#a:Type) (f:a -> bool) (s:seq a) (i:seq_index s):
   Lemma (requires (exists_sat_elems f s /\ i < first_index f s))
         (ensures (not (f (index s i))))
 
 (* Any witness satisfying f implies first_index exists *)
-val lemma_first_index_correct2 (#a:eqtype) (f:a -> bool) (s:seq a) (i:seq_index s):
+val lemma_first_index_correct2 (#a:Type) (f:a -> bool) (s:seq a) (i:seq_index s):
   Lemma (requires (f (index s i)))
         (ensures (exists_sat_elems f s /\ first_index f s <= i))
 
@@ -353,118 +353,123 @@ val lemma_map_extend (#a #b:Type) (f:a -> b) (s:seq a{length s > 0}):
   Lemma (map f s == append1 (map f (prefix s (length s - 1)))
                             (f (index s (length s - 1))))
 
-val zip (#a #b: eqtype) (sa: seq a) (sb: seq b{length sb = length sa}):
+val zip (#a #b: Type) (sa: seq a) (sb: seq b{length sb = length sa}):
   sab: seq (a * b){length sab = length sa}
 
-val lemma_zip_index (#a #b: eqtype) (sa: seq a) (sb: seq b{length sb = length sa}) (i: seq_index sa):
+val lemma_zip_index (#a #b: Type) (sa: seq a) (sb: seq b{length sb = length sa}) (i: seq_index sa):
   Lemma (requires (True))
-        (ensures (fst (index (zip sa sb) i) = index sa i /\
-                  snd (index (zip sa sb) i) = index sb i))
+        (ensures (fst (index (zip sa sb) i) == index sa i /\
+                  snd (index (zip sa sb) i) == index sb i))
         [SMTPat (index (zip sa sb) i)]
 
-val unzip (#a #b: eqtype) (sab: seq (a * b)): sasb: (seq a * seq b)
+val unzip (#a #b: Type) (sab: seq (a * b)): sasb: (seq a * seq b)
   {length (fst sasb) = length sab /\
    length (snd sasb) = length sab}
 
-val lemma_unzip_index (#a #b: eqtype) (sab: seq (a * b)) (i:seq_index sab):
+val lemma_unzip_index (#a #b: Type) (sab: seq (a * b)) (i:seq_index sab):
   Lemma (requires (True))
-        (ensures (fst (index sab i) = index (fst (unzip sab)) i /\
-                  snd (index sab i) = index (snd (unzip sab)) i))
+        (ensures (fst (index sab i) == index (fst (unzip sab)) i /\
+                  snd (index sab i) == index (snd (unzip sab)) i))
         [SMTPat (index (fst (unzip sab)) i); SMTPat (index (snd (unzip sab)) i)]
 
-val lemma_zip_unzip (#a #b: eqtype) (sa: seq a) (sb: seq b{length sb = length sa}):
+val lemma_zip_unzip (#a #b: Type) (sa: seq a) (sb: seq b{length sb = length sa}):
   Lemma (requires (True))
-        (ensures ((sa, sb) = unzip (zip sa sb)))
+        (ensures ((sa, sb) == unzip (zip sa sb)))
 
-val lemma_unzip_extend (#a #b: eqtype) (sab: seq (a * b){length sab > 0}):
-  Lemma (fst (unzip sab) = append1 (fst (unzip (hprefix sab))) (fst (telem sab)) /\
-         snd (unzip sab) = append1 (snd (unzip (hprefix sab))) (snd (telem sab)))
+val lemma_unzip_extend (#a #b: Type) (sab: seq (a * b){length sab > 0}):
+  Lemma (fst (unzip sab) == append1 (fst (unzip (hprefix sab))) (fst (telem sab)) /\
+         snd (unzip sab) == append1 (snd (unzip (hprefix sab))) (snd (telem sab)))
 
 (* attach their index to elements of a sequence *)
 val attach_index (#a:Type) (s:seq a): Tot (seq (nat * a))
 
 val lemma_attach_len (#a:Type) (s: seq a):
   Lemma (requires (True))
-        (ensures (length (attach_index s) = length s))
+        (ensures (length (attach_index s) == length s))
         [SMTPat (attach_index s)]
 
 val lemma_attach_correct (#a:Type) (s:seq a) (i: seq_index s):
   Lemma (requires (True))
         (ensures (length (attach_index s) = length s /\
                   snd (index (attach_index s) i) == index s i /\
-                  fst (index (attach_index s) i) = i))
+                  fst (index (attach_index s) i) == i))
         [SMTPat (index (attach_index s) i)]
 
 (* reduce operation over sequences *)
 val reduce (#a:Type) (#b:Type) (b0: b) (f: a -> b -> b) (s: seq a): Tot b
 
-val lemma_reduce_empty (#a:Type) (#b:eqtype) (b0:b) (f:a -> b -> b):
-  Lemma (reduce b0 f (empty #a) = b0)
+val lemma_reduce_empty (#a:Type) (#b:Type) (b0:b) (f:a -> b -> b):
+  Lemma (reduce b0 f (empty #a) == b0)
 
-val lemma_reduce_prefix (#a:Type) (#b:eqtype) (b0: b) (f: a -> b -> b) (s: seq a) (i:nat{i <= length s}):
-  Lemma (reduce b0 f s = reduce (reduce b0 f (prefix s i)) f (suffix s (length s - i)))
+val lemma_reduce_prefix (#a:Type) (#b:Type) (b0: b) (f: a -> b -> b) (s: seq a) (i:nat{i <= length s}):
+  Lemma (reduce b0 f s == reduce (reduce b0 f (prefix s i)) f (suffix s (length s - i)))
 
-val lemma_reduce_property_closure (#a:Type) (#b:eqtype) (p: b -> bool) (b0:b) (f: a -> b -> b) (s: seq a):
+val lemma_reduce_property_closure_ty (#a:Type) (#b:Type) (p: b -> Type0) (b0:b) (f: a -> b -> b) (s: seq a):
   Lemma (requires (p b0 /\ (forall (x:a). forall (y:b). (p y ==> p (f x y)))))
         (ensures (p (reduce b0 f s)))
 
-val lemma_reduce_identity (#a:Type) (#b:eqtype) (b0: b) (f: a -> b -> b) (s: seq a):
-  Lemma (requires (forall (x:a). f x b0 = b0))
-        (ensures (reduce b0 f s = b0))
+let lemma_reduce_property_closure (#a:Type) (#b:Type) (p: b -> bool) (b0:b) (f: a -> b -> b) (s: seq a)
+  : Lemma (requires (p b0 /\ (forall (x:a). forall (y:b). (p y ==> p (f x y)))))
+          (ensures (p (reduce b0 f s)))
+  = lemma_reduce_property_closure_ty #a #b (fun b -> p b == true) b0 f s
 
-val lemma_reduce_singleton (#a:Type) (#b:eqtype) (b0: b) (f: a -> b -> b) (s: seq a{length s = 1}):
-  Lemma (reduce b0 f s = f (index s 0) b0)
+val lemma_reduce_identity (#a:Type) (#b:Type) (b0: b) (f: a -> b -> b) (s: seq a):
+  Lemma (requires (forall (x:a). f x b0 == b0))
+        (ensures (reduce b0 f s == b0))
 
-val lemma_reduce_append (#a:Type) (#b:eqtype) (b0:b) (f: a -> b -> b) (s: seq a) (x:a):
-  Lemma (reduce b0 f (append1 s x) = f x (reduce b0 f s))
+val lemma_reduce_singleton (#a:Type) (#b:Type) (b0: b) (f: a -> b -> b) (s: seq a{length s = 1}):
+  Lemma (reduce b0 f s == f (index s 0) b0)
 
-val lemma_reduce_append2 (#a:Type) (#b:eqtype) (b0:b) (f: a -> b -> b) (s: seq a{length s > 0}):
-  Lemma (reduce b0 f s = f (index s (length s - 1)) (reduce b0 f (prefix s (length s - 1))))
+val lemma_reduce_append (#a:Type) (#b:Type) (b0:b) (f: a -> b -> b) (s: seq a) (x:a):
+  Lemma (reduce b0 f (append1 s x) == f x (reduce b0 f s))
+
+val lemma_reduce_append2 (#a:Type) (#b:Type) (b0:b) (f: a -> b -> b) (s: seq a{length s > 0}):
+  Lemma (reduce b0 f s == f (index s (length s - 1)) (reduce b0 f (prefix s (length s - 1))))
 
 (* The index of the next entry that satisfies a filter predicate *)
-val next_index_opt (#a:eqtype) (f:a -> bool) (s:seq a) (i:seq_index s):
+val next_index_opt (#a:Type) (f:a -> bool) (s:seq a) (i:seq_index s):
   Tot (option (j:seq_index s{j > i && f (index s j)}))
 
 (* is there a next element in the sequence that satisfies a filter predicate *)
-let has_next (#a:eqtype) (f:a -> bool) (s:seq a) (i:seq_index s): bool = 
+let has_next (#a:Type) (f:a -> bool) (s:seq a) (i:seq_index s): bool = 
   Some? (next_index_opt f s i)
 
-val intro_has_next (#a:eqtype) (f:a -> bool) (s:seq a) (i:seq_index s) (k:seq_index s{i < k /\ f (Seq.index s k)})
+val intro_has_next (#a:Type) (f:a -> bool) (s:seq a) (i:seq_index s) (k:seq_index s{i < k /\ f (Seq.index s k)})
   : Lemma (has_next f s i /\
            Some?.v (next_index_opt f s i) <= k)
 
 (* the next index satisfying a filter predicate *)
-let next_index (#a:eqtype) (f:a -> bool) (s:seq a) (i:seq_index s{has_next f s i}): 
+let next_index (#a:Type) (f:a -> bool) (s:seq a) (i:seq_index s{has_next f s i}): 
   (j:seq_index s{j > i && f (index s j)}) = Some?.v (next_index_opt f s i)
 
 (* The index of the next entry that satisfies a filter predicate *)
-val prev_index_opt (#a:eqtype) (f:a -> bool) (s:seq a) (i:seq_index s):
+val prev_index_opt (#a:Type) (f:a -> bool) (s:seq a) (i:seq_index s):
   Tot (option (j:seq_index s{j < i && f (index s j)}))
 
 (* is there a next element in the sequence that satisfies a filter predicate *)
-let has_prev (#a:eqtype) (f:a -> bool) (s:seq a) (i:seq_index s): bool = 
+let has_prev (#a:Type) (f:a -> bool) (s:seq a) (i:seq_index s): bool = 
   Some? (prev_index_opt f s i)
 
 (* the next index satisfying a filter predicate *)
-let prev_index (#a:eqtype) (f:a -> bool) (s:seq a) (i:seq_index s{has_prev f s i}): 
+let prev_index (#a:Type) (f:a -> bool) (s:seq a) (i:seq_index s{has_prev f s i}): 
   (j:seq_index s{j < i && f (index s j)}) = Some?.v (prev_index_opt f s i)
 
-val filter_snoc (#a:eqtype) (f:a -> bool) (s:seq a) (x:a)
+val filter_snoc (#a:Type) (f:a -> bool) (s:seq a) (x:a)
   : Lemma (if f x 
            then filter f (Seq.snoc s x) `Seq.equal` Seq.snoc (filter f s) x
            else filter f (Seq.snoc s x) `Seq.equal` filter f s)
 
-let filter_map (#a:eqtype) #b 
+let filter_map (#a:Type) #b 
                (filter: a -> bool)
                (f:(refine filter -> b))
                (s:seq a)
    : seq b
    = map f (filter_refine filter s)
 
-val filter_map_emp (#a:eqtype) (#b:Type) (filter: a -> bool) (f:refine filter -> b) 
+val filter_map_emp (#a:Type) (#b:Type) (filter: a -> bool) (f:refine filter -> b) 
   : Lemma (filter_map filter f Seq.empty `Seq.equal` Seq.empty)
   
-let filter_map_snoc (#a:eqtype) (#b:Type)
+let filter_map_snoc (#a:Type) (#b:Type)
                     (filter: a -> bool)
                     (f:refine filter -> b)
                     (s:seq a)
@@ -492,8 +497,8 @@ val each_index_mem (#a: eqtype) (l: seq a) (i: seq_index l)
           [SMTPat (mem (index l i))]
 
 (* a sequence with distinct values *)
-let distinct_elems (#a: eqtype) (s: seq a)
-  = forall (i1 i2: seq_index s). i1 <> i2 ==> (index s i1) <> (index s i2)
+let distinct_elems (#a: Type) (s: seq a)
+  = forall (i1 i2: seq_index s). i1 <> i2 ==> (index s i1) =!= (index s i2)
 
 val distinct_elems_comp (#a: eqtype) (s: seq a)
   : b:bool {b <==> distinct_elems s}
