steel/Zeta.Steel.FormatsManual.fsti
@@ -171,5 +171,5 @@ val serialize_stamped_record : P.serializer spec_serializer_stamped_record
 
 /// This is an ad hoc bound due to a bound on Blake hashable inputs
 val serialized_stamped_record_length (s:stamped_record)
-  : Lemma (Seq.length (spec_serializer_stamped_record s) <= 8192)
+  : Lemma (Seq.length (spec_serializer_stamped_record s) <= 4096)
 
