steel/Zeta.Steel.IArray.fsti
@@ -1,0 +1,125 @@
+module Zeta.Steel.IArray
+open Steel.ST.Util
+open Zeta.Steel.Util
+
+module G = FStar.Ghost
+module Set = FStar.Set
+module Map = FStar.Map
+module U32 = FStar.UInt32
+
+type hash_fn (k:eqtype) = k -> U32.t
+
+val tbl (#k:eqtype)
+        (#v:Type0)
+        (#contents:Type0)
+        (h:hash_fn k)
+        (vp:k -> v -> contents -> vprop)
+  : Type0
+
+let repr (k:eqtype) (contents:Type0) = Map.t k contents
+
+let set_add (s:Set.set 'a) (x:'a) = Set.union s (Set.singleton x)
+let set_remove (s:Set.set 'a) (x:'a) = Set.intersect s (Set.complement (Set.singleton x))
+
+
+(* perm t m b: asserts ownership of the underlying array
+
+       *and* ownership of `vp k v c` for every (k, v)
+             in memory
+             except for those keys in b, that have been borrowed
+
+             The representation map `m` collapses the indirection
+             via v. I.e., it directly associates keys `k`
+             with the contents of `v`.
+*)
+val perm (#k:eqtype)
+         (#v:Type0)
+         (#contents:Type0)
+         (#h:hash_fn k)
+         (#vp: k -> v -> contents -> vprop)
+         (t:tbl h vp)
+         ([@@@smt_fallback] m:repr k contents)
+         ([@@@smt_fallback] borrows:Set.set k)
+  : vprop
+
+let finalizer (#k:eqtype)
+              (#v:Type)
+              (#contents:Type)
+              (vp:k -> v -> contents -> vprop) =
+  x:k -> y:v -> STT unit (exists_ (vp x y)) (fun _ -> emp)
+
+val create (#k:eqtype)
+           (#v:Type0)
+           (#contents:Type0)
+           (#vp: k -> v -> contents -> vprop)
+           (h:hash_fn k)
+           (n:U32.t{U32.v n > 0})
+           (finalize: finalizer vp)
+  : STT (tbl h vp) emp (fun a -> perm a empty_map Set.empty)
+
+
+let get_post (#k:eqtype)
+             (#v:Type0)
+             (#contents:Type0)
+             (#h:hash_fn k)
+             (#vp: k -> v -> contents -> vprop)
+             (m:G.erased (repr k contents))
+             (b:G.erased (Set.set k))
+             (a:tbl h vp)
+             (i:k)
+             (res:option v)
+  : vprop
+  = let c = Map.sel m i in
+    match res with
+    | Some x ->
+      vp i x c `star` perm a m (set_add b i)
+    | _ -> perm a m b
+
+(* Returns the value associated with i and permission to it.
+
+   In this formulation, the rest of the map becomes unusable
+   until permission to the returned value is restored to the map *)
+val get (#k:eqtype)
+        (#v:Type0)
+        (#contents:Type0)
+        (#h:hash_fn k)
+        (#vp: k -> v -> contents -> vprop)
+        (#m:G.erased (repr k contents))
+        (#b:G.erased (Set.set k))
+        (a:tbl h vp)
+        (i:k)
+  : ST (option v)
+       (perm a m b)
+       (get_post m b a i)
+       (requires not (Set.mem i b))
+       (ensures fun o -> Some? o ==> Map.contains m i)
+
+(* If i happens to collide with an existing key i' in memory
+   then then i' is vacated and the finalizer is called on its contents *)
+val put (#k:eqtype)
+        (#v:Type0)
+        (#contents:Type0)
+        (#h:hash_fn k)
+        (#vp: k -> v -> contents -> vprop)
+        (#m:G.erased (repr k contents))
+        (#b:G.erased (Set.set k))
+        (a:tbl h vp)
+        (i:k)
+        (x:v)
+        (c:Ghost.erased contents)
+  : STT unit
+      (perm a m b `star` vp i x c)
+      (fun _ -> perm a (Map.upd m i c) (set_remove b i))
+
+(* Call the finalizer on every value stored in memory
+   and then frees the array itself *)
+val free (#k:eqtype)
+         (#v:Type0)
+         (#h:hash_fn k)
+         (#contents: Type0)
+         (#vp:k -> v -> contents -> vprop)
+         (#m:G.erased (repr k contents))
+         (a:tbl h vp)
+  : STT unit
+      (perm a m Set.empty)
+      (fun _ -> emp)
