steel/Zeta.Steel.Util.fst
@@ -1,0 +1,12 @@
+module Zeta.Steel.Util
+open Steel.ST.Util
+module A = Steel.ST.Array
+module U32 = FStar.UInt32
+let coerce_eq (#a:Type) (#b:Type) (_:squash (a == b)) (x:a) : b = x
+
+let full = Steel.FractionalPermission.full_perm
+let half = Steel.FractionalPermission.half_perm full
+let larray t (n:U32.t) = A.larray t (U32.v n)
+
+assume
+val empty_map (#k:eqtype) (#v:Type) : FStar.Map.t k v
