steel/Zeta.Steel.Verifier.fst
@@ -1,0 +1,607 @@
+module Zeta.Steel.Verifier
+friend Zeta.Steel.VerifierTypes
+open Zeta.Steel.VerifierTypes
+open FStar.Ghost
+open Steel.ST.Util
+module G = Steel.ST.GhostReference
+module R = Steel.ST.Reference
+module A = Steel.ST.Array
+open Zeta.Steel.ApplicationTypes
+module U8 = FStar.UInt8
+module U16 = FStar.UInt16
+module U32 = FStar.UInt32
+module U64 = FStar.UInt64
+open Zeta.Steel.FormatsManual
+open Zeta.Steel.Util
+module T = Zeta.Steel.FormatsManual
+module M = Zeta.Steel.ThreadStateModel
+module AEH = Zeta.Steel.AggregateEpochHashes
+module P = Zeta.Steel.Parser
+
+module Cast = FStar.Int.Cast
+let as_u32 (s:U16.t) : U32.t = Cast.uint16_to_uint32 s
+#push-options "--ide_id_info_off"
+
+let spec_parser_log  = admit()
+
+assume
+val admit__ (#a:Type)
+            (#p:pre_t)
+            (#q:post_t a)
+            (_:unit)
+  : STF a p q True (fun _ -> False)
+
+let finalize_epoch_hash
+  : IArray.finalizer AEH.epoch_hash_perm
+  = fun k v -> drop _ //TODO: Actually free it
+
+let create (tid:T.thread_id)
+  : STT thread_state_t
+    emp
+    (fun t -> thread_state_inv t (M.init_thread_state_model tid))
+  = let failed = R.alloc false in
+    let store : vstore = A.alloc None (as_u32 store_size) in
+    let clock = R.alloc 0uL in
+    let epoch_hashes = IArray.create AEH.epoch_id_hash 64ul finalize_epoch_hash in
+    let processed_entries : G.ref (Seq.seq log_entry_base) = G.alloc Seq.empty in
+    let app_results : G.ref M.app_results = G.alloc Seq.empty in
+    let serialization_buffer = A.alloc 0uy 4096ul in
+    let tsm = M.init_thread_state_model tid in
+    let t : thread_state_t = {
+        thread_id = tid;
+        failed;
+        store;
+        clock;
+        epoch_hashes;
+        processed_entries;
+        app_results;
+        serialization_buffer
+    } in
+    intro_exists _ (A.pts_to serialization_buffer);
+    intro_pure (tsm == M.verify_model tsm Seq.empty);
+    rewrite (R.pts_to failed _ _ `star`
+             A.pts_to store _ `star`
+             R.pts_to clock _ _ `star`
+             IArray.perm epoch_hashes _ _ `star`
+             G.pts_to processed_entries _ _ `star`
+             G.pts_to app_results _ _ `star`
+             exists_ (A.pts_to serialization_buffer) `star`
+             pure _
+            )
+            (thread_state_inv t (M.init_thread_state_model tid));
+    return t
+
+////////////////////////////////////////////////////////////////////////////////
+// Just a couple of warm ups, we don't actually need this
+////////////////////////////////////////////////////////////////////////////////
+#push-options "--query_stats --fuel 0 --ifuel 1"
+
+[@@__reduce__]
+let thread_state_inv' (t:thread_state_t)
+                      ([@@@smt_fallback] tsm:M.thread_state_model)
+  : vprop
+  = R.pts_to t.failed full tsm.failed `star`
+    A.pts_to t.store tsm.store `star`
+    R.pts_to t.clock full tsm.clock `star`
+    IArray.perm t.epoch_hashes tsm.epoch_hashes Set.empty `star`
+    G.pts_to t.processed_entries full tsm.processed_entries `star`
+    G.pts_to t.app_results full tsm.app_results `star`
+    exists_ (A.pts_to t.serialization_buffer)
+
+let intro_thread_state_inv #o
+                           (tsm:M.thread_state_model)
+                           (#f:_)
+                           (#s:_)
+                           (#c:_)
+                           (#eh:_)
+                           (#pe:_)
+                           (#ar:_)
+                           (t:thread_state_t)
+   : STGhost unit o
+     (R.pts_to t.failed full f `star`
+      A.pts_to t.store s `star`
+      R.pts_to t.clock full c `star`
+      IArray.perm t.epoch_hashes eh Set.empty `star`
+      G.pts_to t.processed_entries full pe `star`
+      G.pts_to t.app_results full ar `star`
+      exists_ (A.pts_to t.serialization_buffer))
+     (fun _ -> thread_state_inv' t tsm)
+     (requires
+       tsm.failed == f /\
+       tsm.store == s /\
+       tsm.clock == c /\
+       tsm.epoch_hashes == eh /\
+       tsm.processed_entries == pe /\
+       tsm.app_results == ar)
+     (ensures fun _ ->
+       True)
+   = rewrite (R.pts_to t.failed _ _ `star`
+              A.pts_to t.store _ `star`
+              R.pts_to t.clock _ _ `star`
+              IArray.perm t.epoch_hashes _ _ `star`
+              G.pts_to t.processed_entries _ _ `star`
+              G.pts_to t.app_results _ _ `star`
+              exists_ (A.pts_to t.serialization_buffer))
+             (thread_state_inv' t tsm)
+
+let fail (#tsm:M.thread_state_model)
+         (t:thread_state_t)
+  : STT unit
+    (thread_state_inv' t tsm)
+    (fun _ -> thread_state_inv' t (M.fail tsm))
+  = R.write t.failed true
+
+let vget (#tsm:M.thread_state_model)
+         (t:thread_state_t)
+         (s:slot)
+         (k:key)
+         (v:M.data_value)
+  : STT unit
+    (thread_state_inv' t tsm)
+    (fun _ -> thread_state_inv' t (M.vget tsm s k v))
+  = let se_opt = A.read t.store (as_u32 s) in
+    match se_opt with
+    | None ->
+        R.write t.failed true; ()
+
+    | Some r ->
+        if r.key <> k
+        then (R.write t.failed true; ())
+        else if r.value <> DValue v
+        then (R.write t.failed true; ())
+        else (noop(); ())
+
+let vput (#tsm:M.thread_state_model)
+         (t:thread_state_t)
+         (s:slot)
+         (k:key)
+         (v:M.data_value)
+  : STT unit
+    (thread_state_inv' t tsm)
+    (fun _ -> thread_state_inv' t (M.vput tsm s k v))
+  = let se_opt = A.read t.store (as_u32 s) in
+    match se_opt with
+    | None ->
+      R.write t.failed true; ()
+
+    | Some r ->
+      if r.key <> k
+      then (R.write t.failed true; ())
+      else if not (ApplicationKey? k)
+      then (R.write t.failed true; ())
+      else (A.write t.store (as_u32 s) (Some ({r with M.value = DValue v}));
+            ())
+module KU = Zeta.Steel.KeyUtils
+
+let entry_points_to_some_slot (r:M.store_entry)
+                              (d:bool)
+  : bool
+  = if d
+    then Some? (r.l_child_in_store)
+    else Some? (r.r_child_in_store)
+
+let update_value (#tsm:M.thread_state_model)
+                 (t:thread_state_t)
+                 (s:slot { M.has_slot tsm s })
+                 (r:value { M.is_value_of (M.key_of_slot tsm s) r})
+  : STT unit
+    (thread_state_inv' t tsm)
+    (fun _ -> thread_state_inv' t (M.update_value tsm s r))
+  = let Some v = A.read t.store (as_u32 s) in
+    A.write t.store (as_u32 s) (Some ({v with M.value = r}));
+    ()
+
+let evict_from_store (#tsm:M.thread_state_model)
+                     (t:thread_state_t)
+                     (s:slot)
+                     (s':slot { M.has_slot tsm s' })
+                     (d:bool)
+  : STT unit
+    (thread_state_inv' t tsm)
+    (fun _ -> thread_state_inv' t (M.mevict_from_store tsm s s' d))
+  = let Some r' = A.read t.store (as_u32 s') in
+    let e' =
+        if d
+        then { r' with M.l_child_in_store = None }
+        else { r' with M.r_child_in_store = None }
+    in
+    A.write t.store (as_u32 s') (Some e');
+    A.write t.store (as_u32 s) None;
+    ()
+
+
+let vevictm (#tsm:M.thread_state_model)
+            (t:thread_state_t)
+            (s s':slot_id)
+  : STT unit
+    (thread_state_inv' t tsm)
+    (fun _ -> thread_state_inv' t (M.vevictm tsm s s'))
+  = if not (M.check_slot_bounds s)
+    || not (M.check_slot_bounds s')
+    then (R.write t.failed true; ())
+    else if s = s'
+    then (R.write t.failed true; ())
+    else (
+      let e = A.read t.store (as_u32 s) in
+      let e' = A.read t.store (as_u32 s') in
+      match e, e' with
+      | None, _
+      | _, None -> R.write t.failed true; ()
+      | Some r, Some r' ->
+        let gk = r.M.key in
+        let v = r.M.value in
+        let gk' = r'.M.key in
+        let v' = r'.M.value in
+        let k = M.to_internal_key gk in
+        let k' = M.to_internal_key gk' in
+        (* check k is a proper descendent of k' *)
+        if not (KU.is_proper_descendent k k')
+        then (R.write t.failed true; ())
+        (* check k does not have a (merkle) child in the store *)
+        else if entry_points_to_some_slot r true
+             ||  entry_points_to_some_slot r false
+        then (R.write t.failed true; ())
+        else (
+          let d = KU.desc_dir k k' in
+          let Some v' = M.to_merkle_value v' in
+          let dh' = M.desc_hash_dir v' d in
+          let h = M.hashfn v in
+          match dh' with
+          | T.Dh_vnone _ -> fail t; ()
+          | T.Dh_vsome {T.dhd_key=k2; T.dhd_h=h2; T.evicted_to_blum = b2} ->
+            if k2 <> k then (fail t; ())
+            else if Some? r.M.parent_slot &&
+                    (fst (Some?.v r.M.parent_slot) <> s' ||
+                     snd (Some?.v r.M.parent_slot) <> d)
+            then (fail t; ())
+            else if None? r.M.parent_slot
+                 && entry_points_to_some_slot r' d
+            then (fail t; ())
+            else (
+              let v'_upd = M.update_merkle_value v' d k h false in
+              update_value t s' (T.MValue v'_upd);
+              evict_from_store t s s' d;
+              ()
+            )
+        )
+      )
+
+
+let sat_evictb_checks (#tsm:M.thread_state_model)
+                      (t:thread_state_t)
+                      (s:slot)
+                      (ts:timestamp)
+  : ST bool
+    (thread_state_inv' t tsm)
+    (fun _ -> thread_state_inv' t tsm)
+    (requires True)
+    (ensures fun b -> b == M.sat_evictb_checks tsm s ts)
+  = let ropt = A.read t.store (as_u32 s) in
+    match ropt with
+    | None ->
+      return false
+    | Some r ->
+      let k = r.key in
+      let v = r.value in
+      let clock = R.read t.clock in
+      let b =
+        not (M.is_root_key k) &&
+        (* check time of evict < current time *)
+        clock `M.timestamp_lt` ts &&
+        (* check k has no (merkle) children n the store *)
+        not (entry_points_to_some_slot r true) &&
+        not (entry_points_to_some_slot r false)
+      in
+      return b
+
+module HA = Zeta.Steel.HashAccumulator
+assume
+val ha_add (#v:erased (HA.hash_value_t))
+           (ha:HA.ha)
+           (l:U32.t)
+           (#bs:erased bytes { U32.v l <= Seq.length bs /\ U32.v l <= HA.blake2_max_input_length })
+           (input:A.array U8.t)
+  : STT bool
+       (HA.ha_val ha v `star` A.pts_to input bs)
+       (fun b ->
+         A.pts_to input bs `star`
+         HA.ha_val ha (HA.maybe_aggregate_hashes b v
+                         (HA.hash_one_value (Seq.slice bs 0 (U32.v l)))))
+
+
+let unfold_epoch_hash_perm #o (k:M.epoch_id) (v:AEH.epoch_hashes_t) (c:M.epoch_hash)
+  : STGhost unit o
+    (AEH.epoch_hash_perm k v c)
+    (fun _ ->
+      HA.ha_val v.hadd c.hadd `star`
+      HA.ha_val v.hevict c.hevict)
+    (requires True)
+    (ensures fun _ ->
+      reveal v.complete == c.epoch_complete)
+  = rewrite (AEH.epoch_hash_perm k v c)
+            (HA.ha_val v.hadd c.hadd `star`
+             HA.ha_val v.hevict c.hevict `star`
+             pure (reveal v.complete == c.epoch_complete));
+    elim_pure _
+
+let fold_epoch_hash_perm #o
+                         (k:M.epoch_id)
+                         (v:AEH.epoch_hashes_t)
+                         (#had #hev:HA.hash_value_t)
+                         (c:M.epoch_hash)
+  : STGhost unit o
+    (HA.ha_val v.hadd had `star`
+     HA.ha_val v.hevict hev)
+    (fun _ -> AEH.epoch_hash_perm k v c)
+    (requires
+      c.hadd == had /\
+      c.hevict == hev /\
+      reveal v.complete == c.epoch_complete)
+    (ensures fun _ -> True)
+  = intro_pure (reveal v.complete == c.epoch_complete);
+    rewrite (HA.ha_val v.hadd had `star`
+             HA.ha_val v.hevict hev `star`
+             pure _)
+            (AEH.epoch_hash_perm k v c)
+
+
+
+let maybe_update_hadd (b:bool)
+                      (c:M.epoch_hash)
+                      (r:T.record)
+                      (t:T.timestamp)
+                      (thread_id:T.thread_id)
+  : GTot M.epoch_hash
+  = if b then { c with hadd = M.update_hash_value c.hadd r t thread_id }
+    else c
+
+let maybe_update_hadd_false (tsm:M.thread_state_model)
+                            (e:M.epoch_id)
+                            (r:T.record)
+                            (ts:T.timestamp)
+                            (thread_id:T.thread_id)
+  : Lemma (requires
+            Map.contains tsm.epoch_hashes e)
+          (ensures
+            Map.upd tsm.epoch_hashes e
+                    (maybe_update_hadd false (Map.sel tsm.epoch_hashes e) r ts thread_id) ==
+            tsm.epoch_hashes)
+  = assert (Map.equal tsm.epoch_hashes (Map.upd tsm.epoch_hashes e (Map.sel tsm.epoch_hashes e)))
+
+let tsm_maybe_update_hadd (b:bool)
+                          (tsm:M.thread_state_model)
+                          (e:M.epoch_id)
+                          (r:T.record)
+                          (ts:T.timestamp)
+                          (thread_id:T.thread_id)
+   : M.thread_state_model
+  = if b
+    then let c = Map.sel tsm.epoch_hashes e in
+         {tsm with epoch_hashes =
+                   Map.upd tsm.epoch_hashes
+                      e
+                      (maybe_update_hadd b c r ts thread_id)}
+    else tsm
+
+let tsm_maybe_update_hadd' (b:bool)
+                          (tsm:M.thread_state_model)
+                          (e:M.epoch_id)
+                          (r:T.record)
+                          (ts:T.timestamp)
+                          (thread_id:T.thread_id)
+   : M.thread_state_model
+  = let c = Map.sel tsm.epoch_hashes e in
+    {tsm with epoch_hashes =
+                   Map.upd tsm.epoch_hashes
+                      e
+                      (maybe_update_hadd b c r ts thread_id)}
+
+let tsm_maybe_update_hadd_equiv
+                          (b:bool)
+                          (tsm:M.thread_state_model)
+                          (e:M.epoch_id)
+                          (r:T.record)
+                          (ts:T.timestamp)
+                          (thread_id:T.thread_id)
+  : Lemma (requires
+            Map.contains tsm.epoch_hashes e)
+          (ensures
+            tsm_maybe_update_hadd' b tsm e r ts thread_id ==
+            tsm_maybe_update_hadd b tsm e r ts thread_id)
+  = if b then ()
+    else maybe_update_hadd_false tsm e r ts thread_id
+
+let update_hadd (#tsm:M.thread_state_model)
+                (t:thread_state_t)
+                (e:M.epoch_id)
+                (r:T.record)
+                (ts:T.timestamp)
+                (thread_id:T.thread_id)
+  : STT bool
+    (thread_state_inv' t tsm)
+    (fun b -> thread_state_inv' t (tsm_maybe_update_hadd b tsm e r ts thread_id))
+  = let vopt = IArray.get t.epoch_hashes e in
+    match vopt with
+    | None ->
+      rewrite (IArray.get_post _ _ _ _ vopt)
+              (IArray.perm t.epoch_hashes tsm.epoch_hashes Set.empty);
+      return false
+
+    | Some v ->
+      rewrite (IArray.get_post _ _ _ _ vopt)
+              (AEH.epoch_hash_perm e v (Map.sel tsm.epoch_hashes e) `star`
+               IArray.perm t.epoch_hashes tsm.epoch_hashes (IArray.set_add Set.empty e));
+      unfold_epoch_hash_perm _ _ _;
+      let sr = {
+        record = r;
+        timestamp = ts;
+        thread_id = thread_id
+      } in
+      T.serialized_stamped_record_length sr;
+      let n = T.serialize_stamped_record 4096ul 0ul t.serialization_buffer sr in
+      let bs = elim_exists () in
+      elim_pure ( _ /\ _ /\ _ /\ _);
+      let b = ha_add v.hadd n t.serialization_buffer in
+      fold_epoch_hash_perm e v
+        (maybe_update_hadd b (Map.sel tsm.epoch_hashes e) r ts thread_id);
+      IArray.put t.epoch_hashes e v _;
+      assert (IArray.set_remove (IArray.set_add Set.empty e) e `Set.equal` Set.empty);
+      rewrite (IArray.perm _ _ _)
+              (IArray.perm t.epoch_hashes
+                           (Map.upd tsm.epoch_hashes e
+                                   (maybe_update_hadd b (Map.sel tsm.epoch_hashes e) r ts thread_id))
+                           Set.empty);
+      intro_exists _ (A.pts_to t.serialization_buffer);
+      tsm_maybe_update_hadd_equiv b tsm e r ts thread_id;
+      rewrite (thread_state_inv' t (tsm_maybe_update_hadd' b tsm e r ts thread_id))
+              (thread_state_inv' t (tsm_maybe_update_hadd b tsm e r ts thread_id));
+      return b
+
+// let update_hevict (tsm:thread_state_model)
+//                   (e:epoch_id)
+//                   (r:T.record)
+//                   (t:T.timestamp)
+//                   (thread_id:T.thread_id)
+//   = {tsm with epoch_hashes = update_epoch_hevict tsm.epoch_hashes e r t thread_id }
+
+// let vevictb_update_hash_clock (#tsm:M.thread_state_model)
+//                               (t:thread_state_t)
+//                               (s:slot)
+//                               (ts:timestamp { M.sat_evictb_checks tsm s t })
+//    : STT unit
+//      (thread_state_inv' t tsm)
+//      (fun _ -> thread_state_inv' t (M.vevictb_update_hash_clock tsm s ts))
+//    = let Some r = A.read t.store (as_u32 s) in
+//      let k = r.key in
+//      let v = r.value in
+//      (* update evict hash *)
+
+//      let tsm = update_hevict tsm (epoch_of_timestamp t) (k, v) t tsm.thread_id in
+//      {tsm with clock = t}
+
+// let vevictb (tsm:thread_state_model)
+//             (s:slot_id)
+//             (t:timestamp)
+//   : thread_state_model
+//   = if not (check_slot_bounds s) then fail tsm
+//     else if not (sat_evictb_checks tsm s t)
+//     then fail tsm
+//     else (
+//       let Some r = get_entry tsm s in
+//       if r.add_method <> BAdd
+//       then fail tsm
+//       else (
+//         let tsm = vevictb_update_hash_clock tsm s t in
+//         bevict_from_store tsm s
+//       )
+//     )
+
+// let vevictbm (tsm:thread_state_model)
+//              (s s':slot_id)
+//              (t:timestamp)
+//   : thread_state_model
+//   = if not (check_slot_bounds s)
+//     || not (check_slot_bounds s') then fail tsm
+//     else if s = s' then fail tsm
+//     else if not (sat_evictb_checks tsm s t)
+//     then fail tsm
+//     else if None? (get_entry tsm s')
+//     then fail tsm
+//     else (
+//       let Some r = get_entry tsm s in
+//       let Some r' = get_entry tsm s' in
+//       if r.add_method <> MAdd
+//       then fail tsm
+//       else (
+//         let gk = r.key in
+//         let gk' = r'.key in
+//         let v' = r'.value in
+//         let k = to_internal_key gk in
+//         let k' = to_internal_key gk' in
+//         if not (KU.is_proper_descendent k k')
+//         then fail tsm
+//         else (
+//            let Some mv' = to_merkle_value v' in
+//            let d = KU.desc_dir k k' in
+//            let dh' = desc_hash_dir mv' d in
+//            match dh' with
+//            | T.Dh_vnone _ -> fail tsm
+//            | T.Dh_vsome {T.dhd_key=k2; T.dhd_h=h2; T.evicted_to_blum = b2} ->
+//              if (k2 <> k) || (b2 = T.Vtrue)
+//              then fail tsm
+//              else if None? r.parent_slot
+//                   || fst (Some?.v r.parent_slot) <> s'
+//                   || snd (Some?.v r.parent_slot) <> d
+//              then fail tsm
+//              else (
+//                let tsm = vevictb_update_hash_clock tsm s t in
+//                let mv'_upd = update_merkle_value mv' d k h2 true in
+//                let tsm = update_value tsm s' (MValue mv'_upd) in
+//                mevict_from_store tsm s s' d
+//            )
+//         )
+//       )
+//     )
+
+
+
+
+// let vaddb (#tsm:M.thread_state_model)
+//           (t:thread_state_t)
+//           (s:slot_id)
+//           (ts:T.timestamp)
+//           (tid:T.thread_id)
+//           (p:M.payload)
+//   : STT unit
+//     (thread_state_inv' t tsm)
+//     (fun _ -> thread_state_inv' t (M.vaddb tsm s ts tid p))
+//   = if not (M.check_slot_bounds s)
+//     then (R.write t.failed true; ())
+//     else (
+//       match record_of_payload p with
+//       | None ->
+//         R.write t.failed true; ()
+//         fail tsm //parsing failure
+//       | Some (| k, v |) ->
+//         if is_root_key k
+//         then (fail t; intro_ //root key
+//         else if Some? (get_entry tsm s) then fail tsm //slot is already full
+//         else (
+//         //add hash (k, v, t, thread_id) to hadd.[epoch_of_timestamp t]
+//         let tsm = update_hadd tsm (epoch_of_timestamp t) (k, v) t thread_id in
+//         match next t with //increment the time
+//         | None ->
+//           fail tsm //overflow
+//         | Some t' ->
+//           let tsm = update_clock tsm (max tsm.clock t') in
+//           put_entry tsm s (mk_entry k v BAdd)
+//       )
+
+
+// val serialized_new_app_results (init final:M.app_results)
+//                                (n_out:U32.t)
+//                                (out: P.bytes)
+//   : prop
+
+// let delta_app_results (tsm0 tsm1:M.thread_state_model)
+//   : GTot (Seq.seq M.app_results)
+//   = Prims.admit()
+
+// let bytes_of_app_results (s:Seq.seq M.app_results)
+//   : GTot bytes
+//   = Prims.admit()
+
+// /// Entry point to run a single verifier thread on a log
+let verify (#tsm:M.thread_state_model)
+           (t:thread_state_t) //handle to the thread state
+           (#log_bytes:erased bytes)
+           (#len:U32.t)
+           (log:larray U8.t len) //concrete log
+           (#outlen:U32.t)
+           (out:larray U8.t outlen) //out array, to write outputs
+           (#logrefs: erased (AEH.log_refs_t))
+           (aeh:AEH.aggregate_epoch_hashes logrefs) //lock & handle to the aggregate state
+           (mylogref:AEH.log_ref { //this thread's contribution to the aggregate state
+             Map.sel logrefs tsm.thread_id == mylogref
+            })
+  = admit__()
