steel/Zeta.Steel.VerifierTypes.fst
@@ -1,0 +1,70 @@
+module Zeta.Steel.VerifierTypes
+
+open FStar.Ghost
+open Steel.ST.Util
+module A = Steel.ST.Array
+module R = Steel.ST.Reference
+module G = Steel.ST.GhostReference
+
+open Zeta.Steel.ApplicationTypes
+module U8 = FStar.UInt8
+module U16 = FStar.UInt16
+module U32 = FStar.UInt32
+module U64 = FStar.UInt64
+open Zeta.Steel.ApplicationTypes
+open Zeta.Steel.FormatsManual
+module M = Zeta.Steel.ThreadStateModel
+
+open Zeta.Steel.FormatsManual
+open Zeta.Steel.Util
+module T = Zeta.Steel.FormatsManual
+module M = Zeta.Steel.ThreadStateModel
+module AEH = Zeta.Steel.AggregateEpochHashes
+module IArray = Zeta.Steel.IArray
+module HA = Zeta.Steel.HashAccumulator
+#push-options "--ide_id_info_off"
+
+let vstore
+  : Type0
+  = a:A.array (option M.store_entry) {
+       A.length a == U16.v store_size
+    }
+
+noeq
+type thread_state_t = {
+  thread_id    : T.thread_id;
+  failed       : R.ref bool;
+  store        : vstore;
+  clock        : R.ref U64.t;
+  epoch_hashes : AEH.all_epoch_hashes;
+  processed_entries: G.ref (Seq.seq log_entry_base);
+  app_results  : G.ref M.app_results;
+  serialization_buffer: A.larray U8.t 4096
+}
+
+let thread_id t = t.thread_id
+
+[@@__reduce__]
+let thread_state_inv (t:thread_state_t)
+                     ([@@@smt_fallback] tsm:M.thread_state_model)
+  : vprop
+  = R.pts_to t.failed full tsm.failed `star`
+    A.pts_to t.store tsm.store `star`
+    R.pts_to t.clock full tsm.clock `star`
+    IArray.perm t.epoch_hashes tsm.epoch_hashes Set.empty `star`
+    G.pts_to t.processed_entries full tsm.processed_entries `star`
+    G.pts_to t.app_results full tsm.app_results `star`
+    exists_ (A.pts_to t.serialization_buffer) `star`
+    pure (tsm == M.verify_model
+                   (M.init_thread_state_model t.thread_id)
+                   tsm.processed_entries)
+
+let elim_thread_state_inv (#o:_) (#tsm:M.thread_state_model) (t:thread_state_t)
+  : STGhost unit o
+    (thread_state_inv t tsm)
+    (fun _ -> thread_state_inv t tsm)
+    (requires True)
+    (ensures fun _ ->
+      tsm == M.verify_model (M.init_thread_state_model (thread_id t))
+                            tsm.processed_entries)
+  = extract_pure _
